src/experiments12.lean
@@ -1,0 +1,5 @@
+universe u
+inductive jteq {α : Sort u} (a : α) : α → Prop
+| refl : jteq a
+
+#check @jteq ℕ (3)
